Yatima/Converter/ConvertM.lean
@@ -1,0 +1,53 @@
+import Yatima.Datatypes.Store
+import Yatima.Compiler.Utils
+import Yatima.Converter.ConvertError
+import YatimaStdLib.RBMap
+
+namespace Yatima
+
+namespace Converter
+
+open Std (RBMap)
+
+abbrev RecrCtx := RBMap (Nat × Option Nat) (Nat × Name) compare
+
+structure ConvertEnv where
+  store     : Ipld.Store
+  recrCtx   : RecrCtx
+  bindDepth : Nat
+  deriving Inhabited
+
+def ConvertEnv.init (store : Ipld.Store) : ConvertEnv :=
+  ⟨store, default, 0⟩
+
+structure ConvertState where
+  univ_cache  : RBMap UnivCid Univ compare
+  expr_cache  : RBMap ExprCid Expr compare
+  const_cache : RBMap ConstCid ConstIdx compare
+  defns       : Array Const
+  defnsIdx    : RBMap Name ConstIdx compare
+  deriving Inhabited
+
+abbrev ConvertM := ReaderT ConvertEnv <| EStateM ConvertError ConvertState
+
+def ConvertM.run (env : ConvertEnv) (ste : ConvertState) (m : ConvertM α) :
+    Except ConvertError ConvertState :=
+  match EStateM.run (ReaderT.run m env) ste with
+  | .ok _ stt  => .ok stt
+  | .error e _ => .error e
+
+def ConvertM.unwrap : Option A → ConvertM A :=
+  Option.option (throw .ipldError) pure
+
+def withResetBindDepth : ConvertM α → ConvertM α :=
+  withReader $ fun e => { e with bindDepth := 0 }
+
+def withRecrs (recrCtx : RecrCtx) : ConvertM α → ConvertM α :=
+  withReader $ fun e => { e with recrCtx }
+
+def withNewBind : ConvertM α → ConvertM α :=
+  withReader $ fun e => { e with bindDepth := e.bindDepth + 1 }
+
+namespace Converter
+
+namespace Yatima
